src/named/SimpleProd.v
@@ -6,137 +6,94 @@ Import ListNotations.
 Open Scope string.
 Open Scope list.
 From Utils Require Import Utils.
-From Named Require Import Core Elab SimpleVSubst Matches.
+From Named Require Import Core Elab SimpleSubst Matches.
 Import Core.Notations.
 
 Require Coq.derive.Derive.
 
 Definition prod_lang :=
   [
-     [:> "G" : #"env", "A" : #"ty", "B" : #"ty",
-      "v" : #"val" %"G" %"A",
-      "v'" : #"val" %"G" %"B"
-      ----------------------------------------------- ("ret_pair")
-      #"pair" (#"ret" %"v") (#"ret" %"v'")
-      = #"ret" (#"pair_val" %"v" %"v'")
-      : #"el" %"G" (#"prod" %"A" %"B")
-  ]; 
   [:> "G" : #"env", "A" : #"ty", "B" : #"ty",
-      "e" : #"el" %"G" (#"prod" %"A" %"B"),
+      "e" : #"exp" %"G" (#"prod" %"A" %"B"),
       "G'" : #"env",
       "g" : #"sub" %"G'" %"G"
       ----------------------------------------------- ("proj_2_subst")
-      #"el_subst" %"g" (#".2" %"e")
-      = #".2" (#"el_subst" %"g" %"e")
-      : #"el" %"G'" %"B"
+      #"subst" %"g" (#".2" %"e")
+      = #".2" (#"subst" %"g" %"e")
+      : #"exp" %"G'" %"B"
   ];
   [:> "G" : #"env", "A" : #"ty", "B" : #"ty",
-      "e" : #"el" %"G" (#"prod" %"A" %"B"),
+      "e" : #"exp" %"G" (#"prod" %"A" %"B"),
       "G'" : #"env",
       "g" : #"sub" %"G'" %"G"
       ----------------------------------------------- ("proj_1_subst")
-      #"el_subst" %"g" (#".1" %"e")
-      = #".1" (#"el_subst" %"g" %"e")
-      : #"el" %"G'" %"A"
+      #"subst" %"g" (#".1" %"e")
+      = #".1" (#"subst" %"g" %"e")
+      : #"exp" %"G'" %"A"
   ];
   [:> "G" : #"env", "A" : #"ty", "B" : #"ty",
-      "e" : #"val" %"G" %"A",
-      "e'" : #"val" %"G" %"B",
-      "G'" : #"env",
-      "g" : #"sub" %"G'" %"G"
-      ----------------------------------------------- ("pair_val_subst")
-      #"val_subst" %"g" (#"pair_val" %"e" %"e'")
-      = #"pair_val" (#"val_subst" %"g" %"e") (#"val_subst" %"g" %"e'")
-      : #"val" %"G'" (#"prod" %"A" %"B")
-  ];
-  [:> "G" : #"env", "A" : #"ty", "B" : #"ty",
-      "e" : #"el" %"G" %"A",
-      "e'" : #"el" %"G" %"B",
+      "e" : #"exp" %"G" %"A",
+      "e'" : #"exp" %"G" %"B",
       "G'" : #"env",
       "g" : #"sub" %"G'" %"G"
       ----------------------------------------------- ("pair_subst")
-      #"el_subst" %"g" (#"pair" %"e" %"e'")
-      = #"pair" (#"el_subst" %"g" %"e") (#"el_subst" %"g" %"e'")
-      : #"el" %"G'" (#"prod" %"A" %"B")
+      #"subst" %"g" (#"pair" %"e" %"e'")
+      = #"pair" (#"subst" %"g" %"e") (#"subst" %"g" %"e'")
+      : #"exp" %"G'" (#"prod" %"A" %"B")
+  ];
+  [:> "G" : #"env", "A" : #"ty", "B" : #"ty",
+      "v" : #"exp" %"G" (#"prod" %"A" %"B")
+      ----------------------------------------------- ("prod_eta")
+      #"pair" (#".1" %"v") (#".2" %"v") = %"v"
+      : #"exp" %"G" (#"prod" %"A" %"B")
   ];
   [:> "G" : #"env",
       "A" : #"ty",
       "B" : #"ty",
-      "v1" : #"val" %"G" %"A",
-      "v2" : #"val" %"G" %"B"
+      "v1" : #"exp" %"G" %"A",
+      "v2" : #"exp" %"G" %"B"
       ----------------------------------------------- ("project 2")
-      #".2" (#"ret" (#"pair_val" %"v1" %"v2"))
-      = #"ret" %"v2"
-      : #"el" %"G" %"B"
+      #".2" (#"pair" %"v1" %"v2") = %"v2"
+      : #"exp" %"G" %"B"
   ];
   [:> "G" : #"env",
       "A" : #"ty",
       "B" : #"ty",
-      "v1" : #"val" %"G" %"A",
-      "v2" : #"val" %"G" %"B"
+      "v1" : #"exp" %"G" %"A",
+      "v2" : #"exp" %"G" %"B"
       ----------------------------------------------- ("project 1")
-      #".1" (#"ret" (#"pair_val" %"v1" %"v2"))
-      = #"ret" %"v1"
-      : #"el" %"G" %"A"
+      #".1" (#"pair" %"v1" %"v2") = %"v1"
+      : #"exp" %"G" %"A"
   ];
     [:| "G" : #"env",
       "A" : #"ty",
       "B" : #"ty",
-      "e" : #"el" %"G" (#"prod" %"A" %"B")
+      "e" : #"exp" %"G" (#"prod" %"A" %"B")
       -----------------------------------------------
-      #".2" "e" : #"el" %"G" %"B"
+      #".2" "e" : #"exp" %"G" %"B"
    ];
   [:| "G" : #"env",
       "A" : #"ty",
       "B" : #"ty",
-      "e" : #"el" %"G" (#"prod" %"A" %"B")
+      "e" : #"exp" %"G" (#"prod" %"A" %"B")
       -----------------------------------------------
-      #".1" "e" : #"el" %"G" %"A"
+      #".1" "e" : #"exp" %"G" %"A"
    ];
   [:| "G" : #"env",
       "A" : #"ty",
       "B" : #"ty",
-      "e1" : #"el" %"G" %"A",
-      "e2" : #"el" %"G" %"B"
+      "e1" : #"exp" %"G" %"A",
+      "e2" : #"exp" %"G" %"B"
       -----------------------------------------------
-      #"pair" "e1" "e2" : #"el" %"G" (#"prod" %"A" %"B")
+      #"pair" "e1" "e2" : #"exp" %"G" (#"prod" %"A" %"B")
    ];
-  [:| "G" : #"env",
-      "A" : #"ty",
-      "B" : #"ty",
-      "v1" : #"val" %"G" %"A",
-      "v2" : #"val" %"G" %"B"
-      -----------------------------------------------
-      #"pair_val" "v1" "v2" : #"val" %"G" (#"prod" %"A" %"B")
-    ];
   [:| "A" : #"ty", "B": #"ty"
       -----------------------------------------------
       #"prod" "A" "B" : #"ty"
   ]]%arule.
-
 
 Derive prod_elab
        SuchThat (Pre.elab_lang subst_elab prod_lang prod_elab)
        As prod_wf.
 Proof. auto_elab. Qed.
 #[export] Hint Resolve prod_wf : elab_pfs.
-
-(*Note that because the projections aren't values,
-  we can't put the eta law directly at the value level
-*)
-Definition prod_eta :=
-  [
-     [:> "G" : #"env", "A" : #"ty", "B" : #"ty",
-      "v" : #"val" %"G" (#"prod" %"A" %"B")
-      ----------------------------------------------- ("prod_eta")
-      #"ret" %"v"
-      = #"pair" (#".1" (#"ret" %"v")) (#".2" (#"ret" %"v"))
-      : #"el" %"G" (#"prod" %"A" %"B")
-  ]]%arule.
-
-
-Derive prod_eta_elab
-       SuchThat (Pre.elab_lang (prod_elab ++ subst_elab) prod_eta prod_eta_elab)
-       As prod_eta_wf.
-Proof. auto_elab. Qed.
-#[export] Hint Resolve prod_eta_wf : elab_pfs.
